@prefix :        <http://vocab.dhlab.epfl.ch/data-core#> .
@prefix rdfs:    <http://www.w3.org/2000/01/rdf-schema#> .
@prefix owl:     <http://www.w3.org/2002/07/owl#> .
@prefix xsd:     <http://www.w3.org/2001/XMLSchema#> .
@prefix rdf:     <http://www.w3.org/1999/02/22-rdf-syntax-ns#> .
@prefix core:    <http://vocab.dhlab.epfl.ch/data-core#> .
@prefix skos:    <http://www.w3.org/2004/02/skos/core#> .

core:Source
      a       owl:Class ;
      rdfs:comment "An information object with a digital representation."@en ;
      rdfs:label "Source"@en .

<http://vocab.dhlab.epfl.ch/data-core>
      a       owl:Ontology ;
      rdfs:comment "Core Data Model Ontology"@en , "This ontology defines the core elements of the Venice time machine data model, specifically regarding material of textual nature."@en ;
      owl:versionIRI <http://vocab.dhlab.epfl.ch/data-core/1.0> .

core:Entity
      a       owl:Class ;
      rdfs:comment "Cf. the 'KnowledgeStore Core Data Model ontology' definition \"Any identifiable entity in the domain of discourse, extracted from text and/or imported from some source of background knowledge.\""@en ;
      rdfs:label "Entity"@en ;
      skos:closeMatch "http://dkm.fbk.eu/ontologies/knowledgestore#Entity"^^xsd:anyURI .

skos:closeMatch
      a       owl:AnnotationProperty .

core:Mention
      a       owl:Class ;
      rdfs:comment "Fragment of an information object (source) which refer to an entity."@en ;
      rdfs:label "Mention"@en ;
      skos:closeMatch "http://dkm.fbk.eu/ontologies/knowledgestore#Mention"^^xsd:anyURI .

core:isMentionedIn
      a       owl:ObjectProperty ;
      rdfs:comment "This property indicates the source were a mention occurs."@en ;
      rdfs:domain core:Mention ;
      rdfs:label "isMentionedIn"@en ;
      rdfs:range core:Source .

core:isComponentOf
      a       owl:ObjectProperty ;
      rdfs:isDefinedBy "http://www.ontologydesignpatterns.org/cp/owl/componency.owl#isComponentOf"^^xsd:anyURI ;
      rdfs:label "isComponentOf"@en .

core:hasComponent
      a       owl:ObjectProperty ;
      rdfs:isDefinedBy "http://www.ontologydesignpatterns.org/cp/owl/componency.owl#hasComponent"^^xsd:anyURI ;
      rdfs:label "hasComponent"@en ;
      owl:inverseOf core:isComponentOf .

core:refersTo
      a       owl:FunctionalProperty , owl:ObjectProperty ;
      rdfs:comment "This property indicates the entity a mention refers to."@en ;
      rdfs:domain core:Mention ;
      rdfs:label "refersTo"@en ;
      rdfs:range core:Entity .

core:referredBy
      a       owl:ObjectProperty ;
      rdfs:comment "This property indicates the mention an entity is referred by."@en ;
      rdfs:domain core:Entity ;
      rdfs:label "referredBy"@en ;
      rdfs:range core:Mention ;
      owl:inverseOf core:refersTo .

core:hasMention
      a       owl:ObjectProperty ;
      rdfs:comment "This property indicates the mention which occur in a source."@en ;
      rdfs:domain core:Source ;
      rdfs:label "hasMention"@en ;
      rdfs:range core:Mention ;
      owl:inverseOf core:isMentionedIn .
