@prefix :        <http://vocab.dhlab.epfl.ch/vtm-core#> .
@prefix rdfs:    <http://www.w3.org/2000/01/rdf-schema#> .
@prefix owl:     <http://www.w3.org/2002/07/owl#> .
@prefix xsd:     <http://www.w3.org/2001/XMLSchema#> .
@prefix rdf:     <http://www.w3.org/1999/02/22-rdf-syntax-ns#> .
@prefix skos:    <http://www.w3.org/2004/02/skos/core#> .

<http://vocab.dhlab.epfl.ch/data-core#Source>
      a       owl:Class ;
      rdfs:comment "An information object with a digital representation."@en .

<http://vocab.dhlab.epfl.ch/data-core>
      a       owl:Ontology ;
      rdfs:comment "This ontology defines the core elements of the Venice time machine data model, regarding specifically material of textual nature."@en ;
      owl:versionIRI <http://vocab.dhlab.epfl.ch/data-core/1.0> .

<http://vocab.dhlab.epfl.ch/data-core#Entity>
      a       owl:Class ;
      rdfs:comment "Cf. Knowledge store definition \"Any identifiable entity in the domain of discourse, extracted from text and/or imported from some source of background knowledge.\""@en ;
      skos:closeMatch "http://dkm.fbk.eu/ontologies/knowledgestore#Entity"^^xsd:anyURI .

skos:closeMatch
      a       owl:AnnotationProperty .

<http://vocab.dhlab.epfl.ch/data-core#Mention>
      a       owl:Class ;
      rdfs:comment "Fragment of an information object (source) which refer to an entity."@en ;
      skos:closeMatch "http://dkm.fbk.eu/ontologies/knowledgestore#Mention"^^xsd:anyURI .

<http://vocab.dhlab.epfl.ch/data-core#isMentionedIn>
      a       owl:ObjectProperty ;
      rdfs:comment "Tjis property indicates the source were a mention occurs."@en ;
      rdfs:domain <http://vocab.dhlab.epfl.ch/data-core#Mention> ;
      rdfs:range <http://vocab.dhlab.epfl.ch/data-core#Source> .

<http://vocab.dhlab.epfl.ch/data-core#isComponentOf>
      a       owl:ObjectProperty ;
      rdfs:isDefinedBy "http://www.ontologydesignpatterns.org/cp/owl/componency.owl#isComponentOf"^^xsd:anyURI .

<http://vocab.dhlab.epfl.ch/data-core#hasComponent>
      a       owl:ObjectProperty ;
      rdfs:isDefinedBy "http://www.ontologydesignpatterns.org/cp/owl/componency.owl#hasComponent"^^xsd:anyURI ;
      owl:inverseOf <http://vocab.dhlab.epfl.ch/data-core#isComponentOf> .

<http://vocab.dhlab.epfl.ch/data-core#refersTo>
      a       owl:FunctionalProperty , owl:ObjectProperty ;
      rdfs:comment "This property indicates the entity a mention refers to."@en ;
      rdfs:domain <http://vocab.dhlab.epfl.ch/data-core#Mention> ;
      rdfs:range <http://vocab.dhlab.epfl.ch/data-core#Entity> .

<http://vocab.dhlab.epfl.ch/data-core#referredBy>
      a       owl:ObjectProperty ;
      rdfs:comment "This property indicates the mention an entity is referred by."@en ;
      rdfs:domain <http://vocab.dhlab.epfl.ch/data-core#Entity> ;
      rdfs:range <http://vocab.dhlab.epfl.ch/data-core#Mention> ;
      owl:inverseOf <http://vocab.dhlab.epfl.ch/data-core#refersTo> .

<http://vocab.dhlab.epfl.ch/data-core#hasMention>
      a       owl:ObjectProperty ;
      rdfs:comment "This property indicates the mention which occur in a source."@en ;
      rdfs:domain <http://vocab.dhlab.epfl.ch/data-core#Source> ;
      rdfs:range <http://vocab.dhlab.epfl.ch/data-core#Mention> ;
      owl:inverseOf <http://vocab.dhlab.epfl.ch/data-core#isMentionedIn> .
